turn Es & Ds into E & D

spc/RobustIndexedInvariants.v
@@ -1,14 +1,14 @@
 From stdpp Require Import coPset gmap namespaces.
-From sflib Require Import sflib.
+Require Import sflib.
 From iris Require Import bi.big_op.
 From iris Require base_logic.lib.invariants.
 
 Require Import Coqlib PCM PCMAux IProp IPM.
 Require Import Coq.Logic.ClassicalEpsilon.
 
-Local Notation world_id := positive.
+Local Notation univ_id := positive.
 Local Notation level := nat.
-  
+
 Section INDEXED_INVARIANT_SET.
 
   Context `{Σ : GRA.t}.
@@ -19,93 +19,89 @@ Section INDEXED_INVARIANT_SET.
   Definition InvSetRA (sProp : level -> Type) (n : level) : URA.t :=
     (Auth.t (positive ==> URA.agree (sProp n)))%ra.
 
-  Definition OwnIsRA (sProp : level -> Type) : URA.t :=
-    URA.pointwise world_id (@URA.pointwise_dep level (InvSetRA sProp)).
+  Definition OwnIRA (sProp : level -> Type) : URA.t :=
+    URA.pointwise univ_id (@URA.pointwise_dep level (InvSetRA sProp)).
 
-  Definition OwnEsRA : URA.t :=
-    URA.pointwise world_id (URA.pointwise level CoPset.t).
+  Definition OwnERA : URA.t :=
+    URA.pointwise univ_id (CoPset.t).
   
-  Definition OwnDsRA : URA.t :=
-    URA.pointwise world_id (URA.pointwise level (Auth.t Gset.t)).
+  Definition OwnDRA : URA.t :=
+    URA.pointwise univ_id (Auth.t Gset.t).
 
 End INDEXED_INVARIANT_SET.
 
 Section PCM_OWN.
 
   Context `{Σ : GRA.t}.
-
-  Definition OwnI {sProp} `{@GRA.inG (OwnIsRA sProp) Σ} (u: world_id) (n : level) (i : positive) (p : sProp n) :=
-    OwnM (maps_to_res u (@maps_to_res_dep level (@InvSetRA sProp)
-          n (Auth.white (@maps_to_res positive (URA.agree (sProp n)) i (Some (Some p))))) : OwnIsRA sProp).
-
-  Definition OwnI_authR {sProp} `{@GRA.inG (OwnIsRA sProp) Σ} (u: world_id) (n : level) (I : gmap positive (sProp n)) : OwnIsRA sProp :=
-    maps_to_res u (@maps_to_res_dep level _ n (@Auth.black (positive ==> URA.agree (sProp n))%ra
-                                                 (fun i => Some <$> (I !! i)))).
-
-  Definition OwnI_auth {sProp} `{@GRA.inG (OwnIsRA sProp) Σ} (u: world_id) (n: level) (I : gmap positive (sProp n)) :=
-    OwnM (OwnI_authR u n I).
+  Context `{@GRA.inG (OwnIRA sProp) Σ}.
   
-  Definition OwnE `{@GRA.inG OwnEsRA Σ} (u: world_id) (n : level) (E : coPset) :=
-    OwnM (maps_to_res u (@maps_to_res level CoPset.t n (Some E)) : OwnEsRA).
+  Definition OwnIR (u: univ_id) (n : level) (i : positive) (p : sProp n) : OwnIRA sProp :=
+    maps_to_res u (@maps_to_res_dep level (@InvSetRA sProp)
+      n (Auth.white (@maps_to_res positive (URA.agree (sProp n)) i (Some (Some p))))).
+  
+  Definition OwnI (u: univ_id) (n : level) (i : positive) (p : sProp n) :=
+    OwnM (OwnIR u n i p).
 
-  Definition OwnD `{@GRA.inG OwnDsRA Σ} (u: world_id) (n : level) (D: gset positive) :=
-    OwnM (maps_to_res u (@maps_to_res level (Auth.t Gset.t) n (Auth.white (Some D: Gset.t))) : OwnDsRA).
+  Definition OwnI_authR (u: univ_id) (n : level) (I : gmap positive (sProp n)) : OwnIRA sProp :=
+    maps_to_res u (@maps_to_res_dep level _
+      n (@Auth.black (positive ==> URA.agree (sProp n))%ra (fun i => Some <$> (I !! i)))).
 
-  Definition OwnD_authR `{@GRA.inG OwnDsRA Σ} (u: world_id) (n : level) (D: gset positive) : OwnDsRA :=
-    maps_to_res u (@maps_to_res level (Auth.t Gset.t) n (Auth.black (Some D : Gset.t))).
+  Definition OwnI_auth (u: univ_id) (n: level) (I : gmap positive (sProp n)) :=
+    OwnM (OwnI_authR u n I).
 
-  Definition OwnD_auth `{@GRA.inG OwnDsRA Σ} (u: world_id) (n : level): iProp :=
-    (∃ D, OwnM (OwnD_authR u n D))%I.
+  Context `{@GRA.inG OwnERA Σ}.
+   
+  Definition OwnER (u: univ_id) (E: coPset) : OwnERA :=
+    @maps_to_res _ CoPset.t u (Some E).
+  
+  Definition OwnE (u: univ_id) (E: coPset) : iProp :=
+    OwnM (OwnER u E).
 
-  Lemma OwnE_level_diff `{@GRA.inG OwnEsRA Σ} u n1 n2 (E : coPset) :
-    (E <> ∅) -> OwnE u n1 E ∗ OwnE u n2 E ⊢ ⌜n1 <> n2⌝.
-  Proof.
-    intros NEMP.
-    iIntros "[H1 H2]". iCombine "H1 H2" as "H". iPoseProof (OwnM_valid with "H") as "%WF".
-    iPureIntro. intros EQ. subst n2.
-    rewrite /URA.wf /URA.add in WF. unseal "ra". ss. specialize (WF u).
-    rewrite /URA.wf /URA.add in WF. unseal "ra". ss. specialize (WF n1).
-    unfold maps_to_res in WF. des_ifs.
-    rewrite /URA.wf /URA.add in WF. unseal "ra". ss. des_ifs. set_solver.
-  Qed.
+  Context `{@GRA.inG OwnDRA Σ}.
+   
+  Definition OwnDR (u: univ_id) (D: gset positive) : OwnDRA :=
+    maps_to_res u (Auth.white (Some D: Gset.t)).
+  
+  Definition OwnD (u: univ_id) (D: gset positive) :=
+    OwnM (OwnDR u D).
 
-  Lemma OwnE_exploit `{@GRA.inG OwnEsRA Σ} u n (E1 E2 : coPset) :
-    OwnE u n E1 ∗ OwnE u n E2 ⊢ ⌜E1 ## E2⌝.
+  Definition OwnD_authR  (u: univ_id) (D: gset positive) : OwnDRA :=
+    maps_to_res u (Auth.black (Some D : Gset.t)).
+
+  Definition OwnD_auth `{@GRA.inG OwnDRA Σ} (u: univ_id) : iProp :=
+    (∃ D, OwnM (OwnD_authR u D))%I.
+
+  Lemma OwnE_exploit `{@GRA.inG OwnERA Σ} u (E1 E2 : coPset) :
+    OwnE u E1 ∗ OwnE u E2 ⊢ ⌜E1 ## E2⌝.
   Proof.
     iIntros "[H1 H2]". iCombine "H1 H2" as "H". iPoseProof (OwnM_valid with "H") as "%WF".
     iPureIntro.
-    rewrite /URA.wf /URA.add in WF. unseal "ra". ss. specialize (WF u).
-    rewrite /URA.wf /URA.add in WF. unseal "ra". ss. specialize (WF n).
-    unfold maps_to_res in WF. des_ifs.
-    rewrite /URA.wf /URA.add in WF. unseal "ra". ss; des_ifs.
+    rewrite /URA.wf /URA.add /OwnER /maps_to_res in WF. unseal "ra". ss. specialize (WF u).
+    des_ifs. rewrite /URA.wf /URA.add in WF. unseal "ra". ss; des_ifs.
   Qed.
 
-  Lemma OwnE_union `{@GRA.inG OwnEsRA Σ} u n (E1 E2 : coPset) :
-    OwnE u n E1 ∗ OwnE u n E2 ⊢ OwnE u n (E1 ∪ E2).
+  Lemma OwnE_union `{@GRA.inG OwnERA Σ} u (E1 E2 : coPset) :
+    OwnE u E1 ∗ OwnE u E2 ⊢ OwnE u (E1 ∪ E2).
   Proof.
     iIntros "H". iPoseProof (OwnE_exploit with "H") as "%D".
     iRevert "H". iApply from_sep. eapply from_sep_ownM.
-    unfold IsOp, maps_to_res, URA.add. ss. unseal "ra".
-    extensionalities u' n'. des_ifs; ss.
-    - repeat (unfold URA.add; unseal "ra"; ss; des_ifs).
-    - unfold URA.add. unseal "ra". ss. des_ifs. r_solve.
-    - rewrite URA.unit_id. auto.
+    unfold IsOp, OwnER, maps_to_res, URA.add. ss. unseal "ra".
+    extensionalities u'. des_ifs; ss; r_solve.
+    repeat (unfold URA.add; unseal "ra"; ss; des_ifs).
   Qed.
 
-  Lemma OwnE_disjoint `{@GRA.inG OwnEsRA Σ} u n (E1 E2 : coPset) :
-    E1 ## E2 -> OwnE u n (E1 ∪ E2) ⊢ OwnE u n E1 ∗ OwnE u n E2.
+  Lemma OwnE_disjoint `{@GRA.inG OwnERA Σ} u (E1 E2 : coPset) :
+    E1 ## E2 -> OwnE u (E1 ∪ E2) ⊢ OwnE u E1 ∗ OwnE u E2.
   Proof.
     i. unfold OwnE.
     iApply into_sep. eapply into_sep_ownM.
-    unfold IsOp, maps_to_res, URA.add. ss. unseal "ra".
-    extensionalities u' n'. des_ifs.
-    - repeat (unfold URA.add; unseal "ra"; ss; des_ifs).
-    - unfold URA.add. unseal "ra". ss. des_ifs. r_solve.
-    - rewrite URA.unit_id. auto.
+    unfold IsOp, OwnER, maps_to_res, URA.add. ss. unseal "ra".
+    extensionalities u'. des_ifs; r_solve.
+    repeat (unfold URA.add; unseal "ra"; ss; des_ifs).
   Qed.
 
-  Lemma OwnE_subset `{@GRA.inG OwnEsRA Σ} u n (E1 E2 : coPset) :
-    E1 ⊆ E2 -> OwnE u n E2 ⊢ OwnE u n E1 ∗ (OwnE u n E1 -∗ OwnE u n E2).
+  Lemma OwnE_subset `{@GRA.inG OwnERA Σ} u (E1 E2 : coPset) :
+    E1 ⊆ E2 -> OwnE u E2 ⊢ OwnE u E1 ∗ (OwnE u E1 -∗ OwnE u E2).
   Proof.
     iIntros (SUB) "E".
     assert (E2 = E1 ∪ E2 ∖ E1) as EQ.
@@ -116,10 +112,10 @@ Section PCM_OWN.
     iApply OwnE_union. iFrame.
   Qed.
 
-  Global Instance OwnI_persistent {sProp} `{@GRA.inG (OwnIsRA sProp) Σ}
+  Global Instance OwnI_persistent 
     u n i p : Persistent (OwnI u n i p).
   Proof.
-    unfold OwnI.
+    unfold OwnI, OwnIR.
     remember (@maps_to_res_dep level (InvSetRA sProp) n (Auth.white (@maps_to_res positive (URA.agree (sProp n)) i (Some (Some p))))) as r.
     unfold Persistent. iIntros "H".
     iPoseProof (@OwnM_persistently _ _ H _ with "H") as "#HP". iModIntro.
@@ -134,17 +130,17 @@ Section WORLD_SATISFACTION.
   Context `{Σ : GRA.t}.
   Context `{sProp : level -> Type}.
   Context `{@IInvSet Σ sProp}.
-  Context `{@GRA.inG OwnEsRA Σ}.
-  Context `{@GRA.inG OwnDsRA Σ}.
-  Context `{@GRA.inG (OwnIsRA sProp) Σ}.
+  Context `{@GRA.inG OwnERA Σ}.
+  Context `{@GRA.inG OwnDRA Σ}.
+  Context `{@GRA.inG (OwnIRA sProp) Σ}.
 
-  Variable u : world_id.
+  Variable u : univ_id.
   Variable n : level.
 
   Definition inv_satall (I : gmap positive (sProp n)) :=
-    ([∗ map] i ↦ p ∈ I, (prop n p ∗ OwnD u n {[i]}) ∨ OwnE u n {[i]})%I.
+    ([∗ map] i ↦ p ∈ I, (prop n p ∗ OwnD u {[i]}) ∨ OwnE u {[i]})%I.
 
-  Definition wsat : iProp := (OwnD_auth u n ∗ ∃ I, OwnI_auth u n I ∗ inv_satall I)%I.
+  Definition wsat : iProp := (∃ I, OwnI_auth u n I ∗ inv_satall I)%I.
 
   Lemma alloc_name φ
         (INF : forall (E : level -> option (gset positive)) n,
@@ -152,16 +148,16 @@ Section WORLD_SATISFACTION.
             | None => True
             | Some G => (exists i, i ∉ G /\ φ i)
             end)
-    : OwnD_auth u n ⊢ |==>  OwnD_auth u n ∗ ∃ i, ⌜φ i⌝ ∧ OwnD u n {[i]}.
+    : OwnD_auth u ⊢ |==>  OwnD_auth u ∗ ∃ i, ⌜φ i⌝ ∧ OwnD u {[i]}.
   Proof.
     iIntros "[% DA]". specialize (INF (fun _ => Some D) n). ss. des.
     assert (@URA.updatable
-              OwnDsRA
-              (maps_to_res u (maps_to_res n (Auth.black (Some D : Gset.t))))
-              ((maps_to_res u (maps_to_res n (Auth.black (Some (D ∪ {[i]}) : Gset.t))))
-                 ⋅
-                 (maps_to_res u (maps_to_res n (Auth.white (Some {[i]} : Gset.t)))))) as UPD.
-    { rewrite !maps_to_res_add. do 2 apply maps_to_res_updatable.
+              OwnDRA
+              (maps_to_res u (Auth.black (Some D : Gset.t)))
+              ((maps_to_res u (Auth.black (Some (D ∪ {[i]}) : Gset.t)))
+               ⋅
+               (maps_to_res u (Auth.white (Some {[i]} : Gset.t))))) as UPD.
+    { rewrite !maps_to_res_add. apply maps_to_res_updatable.
       ii. ur in H3. des_ifs. des. rewrite URA.unit_idl in H3.
       unfold URA.extends in H3. des. ur in H3.
       ur. rewrite URA.unit_idl. split.
@@ -185,7 +181,7 @@ Section WORLD_SATISFACTION.
             | None => True
             | Some G => (exists i, i ∉ G /\ φ i)
             end)
-    : wsat ⊢ |==> (∃ i, ⌜φ i⌝ ∧ OwnI u n i p) ∗ (prop n p -∗ wsat).
+    : OwnD_auth u ∗ wsat ⊢ |==> (∃ i, ⌜φ i⌝ ∧ OwnI u n i p) ∗ OwnD_auth u ∗ (prop n p -∗ wsat).
   Proof.
     iIntros "[DA [% [AUTH SAT]]]".
     iMod (alloc_name (fun i => i ∉ dom I /\ φ i) with "DA") as "[DA [% [[%iI %iφ] D]]]".
@@ -199,10 +195,10 @@ Section WORLD_SATISFACTION.
     pose (<[i:=p]> I) as I'.
 
     assert (URA.updatable
-              (maps_to_res u (maps_to_res_dep n (@Auth.black (positive ==> URA.agree (sProp n))%ra (fun i => Some <$> (I !! i)))): OwnIsRA sProp)
-              ((maps_to_res u (maps_to_res_dep n (@Auth.black (positive ==> URA.agree (sProp n))%ra (fun i => Some <$> (I' !! i)))): OwnIsRA sProp)
+              (maps_to_res u (maps_to_res_dep n (@Auth.black (positive ==> URA.agree (sProp n))%ra (fun i => Some <$> (I !! i)))): OwnIRA sProp)
+              ((maps_to_res u (maps_to_res_dep n (@Auth.black (positive ==> URA.agree (sProp n))%ra (fun i => Some <$> (I' !! i)))): OwnIRA sProp)
                ⋅
-               (maps_to_res u (maps_to_res_dep n (Auth.white (@maps_to_res _ (URA.agree (sProp n)) i (Some (Some p))))): OwnIsRA sProp))).
+               (maps_to_res u (maps_to_res_dep n (Auth.white (@maps_to_res _ (URA.agree (sProp n)) i (Some (Some p))))): OwnIRA sProp))).
     { setoid_rewrite maps_to_res_add. setoid_rewrite maps_to_res_dep_add.
       apply maps_to_res_updatable. apply maps_to_res_dep_updatable.
       apply Auth.auth_alloc. ii. des. rewrite URA.unit_idl in FRAME. subst. split.
@@ -219,7 +215,7 @@ Section WORLD_SATISFACTION.
 
     iSplit.
     - iExists i. iFrame. ss.
-    - iIntros "P". unfold wsat. iFrame. iExists I'. iFrame.
+    - iFrame. iIntros "P". unfold wsat. iExists I'. iFrame.
       unfold inv_satall. subst I'.
       iApply big_sepM_insert.
       { apply not_elem_of_dom_1; ss. }
@@ -232,17 +228,17 @@ Section WORLD_SATISFACTION.
             | None => True
             | Some G => (exists i, i ∉ G /\ φ i)
             end)
-    : wsat ∗ prop n p ⊢ |==> (∃ i, ⌜φ i⌝ ∧ OwnI u n i p) ∗ wsat.
+    : OwnD_auth u ∗ wsat ∗ prop n p ⊢ |==> (∃ i, ⌜φ i⌝ ∧ OwnI u n i p) ∗ OwnD_auth u ∗ wsat.
   Proof.
-    iIntros "[W P]".
-    iMod (wsat_OwnI_alloc_gen with "W") as "[I W]". eauto.
+    iIntros "(D & W & P)".
+    iMod (wsat_OwnI_alloc_gen with "[D W]") as "(I & D & W)". eauto. iFrame.
     iFrame. iModIntro. iApply "W". iFrame.
   Qed.
 
   Lemma wsat_OwnI_open i p :
-    OwnI u n i p ∗ wsat ∗ OwnE u n {[i]} ⊢ |==> prop n p ∗ wsat ∗ OwnD u n {[i]}.
+    OwnI u n i p ∗ wsat ∗ OwnE u {[i]} ⊢ |==> prop n p ∗ wsat ∗ OwnD u {[i]}.
   Proof.
-    iIntros "(I & [DA [% [AUTH SAT]]] & EN)". iModIntro.
+    iIntros "(I & [% [AUTH SAT]] & EN)". iModIntro.
     unfold OwnI, OwnI_auth, inv_satall.
     iCombine "AUTH I" as "AUTH".
     iPoseProof (OwnM_valid with "AUTH") as "%WF".
@@ -263,9 +259,9 @@ Section WORLD_SATISFACTION.
     iDestruct "AUTH" as "[AUTH I]".
     iPoseProof (big_sepM_delete _ _ _ _ Hip with "SAT") as "[[[H1 H2]|H1] SAT]".
     2: { iCombine "EN H1" as "F". iPoseProof (OwnM_valid with "F") as "%WF".
-         exfalso. unfold maps_to_res, URA.wf, URA.add in WF. unseal "ra". ss.
+         exfalso. unfold OwnER, maps_to_res, URA.wf, URA.add in WF. unseal "ra". ss.
          specialize (WF u). unfold URA.wf, URA.add in WF. unseal "ra". ss.
-         specialize (WF n). des_ifs. unfold URA.wf, URA.add in WF. unseal "ra".
+         des_ifs. unfold URA.wf, URA.add in WF. unseal "ra".
          ss. des_ifs. set_solver.
     }
     iFrame. unfold wsat. iExists I. iFrame. unfold inv_satall.
@@ -273,9 +269,9 @@ Section WORLD_SATISFACTION.
   Qed.
 
   Lemma wsat_OwnI_close i p :
-    OwnI u n i p ∗ wsat ∗ prop n p ∗ OwnD u n {[i]} ⊢ |==> wsat ∗ OwnE u n {[i]}.
+    OwnI u n i p ∗ wsat ∗ prop n p ∗ OwnD u {[i]} ⊢ |==> wsat ∗ OwnE u {[i]}.
   Proof.
-    iIntros "(I & [DA [% [AUTH SAT]]] & P & DIS)". iModIntro.
+    iIntros "(I & [% [AUTH SAT]] & P & DIS)". iModIntro.
     unfold OwnI, OwnI_auth, inv_satall.
     iCombine "AUTH I" as "AUTH".
     iPoseProof (OwnM_valid with "AUTH") as "%WF".
@@ -297,25 +293,19 @@ Section WORLD_SATISFACTION.
     iDestruct "AUTH" as "[AUTH I]".
     iPoseProof (big_sepM_delete _ _ _ _ Hip with "SAT") as "[[[H1 H2]|H1] SAT]".
     { iCombine "DIS H2" as "F". iPoseProof (OwnM_valid with "F") as "%WF".
-      exfalso. unfold maps_to_res, URA.wf, URA.add in WF. unseal "ra". ss.
-      specialize (WF u). unfold URA.wf, URA.add in WF. unseal "ra". ss.
-      specialize (WF n). des_ifs.
-      unfold URA.wf, URA.add in WF. unseal "ra". ss.
-      ur in WF. des_ifs. set_solver.
+      exfalso. unfold OwnDR, maps_to_res, URA.wf, URA.add in WF. unseal "ra". ss.
+      specialize (WF u). unfold URA.wf, URA.add in WF. unseal "ra".
+      des_ifs. ur in WF. ur in WF. des_ifs. set_solver.
     }
     iFrame. unfold wsat. iExists I. iFrame. unfold inv_satall.
     iApply (big_sepM_delete _ _ _ _ Hip). iFrame. iLeft. iFrame.
   Qed.
 
   Lemma wsat_init :
-    OwnM (maps_to_res u (maps_to_res n (Auth.black (Some ∅ : Gset.t))) : OwnDsRA)
-    ∗
-    OwnM (maps_to_res u (maps_to_res_dep n (@Auth.black (positive ==> URA.agree (sProp n))%ra (fun (i : positive) => None))) : OwnIsRA _)
-    ⊢ wsat.
+    OwnI_auth u n ∅ ⊢ wsat.
   Proof.
-    iIntros "[H1 H2]". iSplitL "H1".
-    { iExists ∅. iFrame. }
-    { iExists ∅. iFrame. unfold inv_satall. iApply big_sepM_empty. ss. }
+    iIntros "H".
+    iExists ∅. iFrame. unfold inv_satall. iApply big_sepM_empty. ss.
   Qed.
 
 End WORLD_SATISFACTION.
@@ -405,30 +395,16 @@ Section UNIVERSE.
 
 End UNIVERSE.
 
-Notation coPsets := (gmap level coPset).
-
 Section WSATS.
 
   Context `{Σ : GRA.t}.
   Context `{sProp : level -> Type}.
   Context `{@IInvSet Σ sProp}.
-  Context `{@GRA.inG OwnEsRA Σ}.
-  Context `{@GRA.inG OwnDsRA Σ}.
-  Context `{@GRA.inG (OwnIsRA sProp) Σ}.
+  Context `{@GRA.inG OwnERA Σ}.
+  Context `{@GRA.inG OwnDRA Σ}.
+  Context `{@GRA.inG (OwnIRA sProp) Σ}.
 
-  Definition OwnD_restR (u: world_id) (b: level) : OwnDsRA :=
-    fun u' n =>
-      if (u' =? u)%positive
-      then
-        (if (lt_dec n b)
-         then ε
-         else Auth.black (Some ∅ : Gset.t))
-      else
-        ε.
-
-  Definition OwnD_rest u b := OwnM (OwnD_restR u b)%I.
-
-  Definition OwnI_restR u b : OwnIsRA sProp :=
+  Definition OwnI_restR u b : OwnIRA sProp :=
     fun u' n =>
       if (u' =? u)%positive
       then
@@ -439,59 +415,32 @@ Section WSATS.
         ε.
 
   Definition OwnI_rest u b := OwnM (OwnI_restR u b)%I.
-  
-  Definition OwnE_restR u (Es : coPsets) : OwnEsRA :=
-    fun u' n' =>
-      if (u' =? u)%positive
-      then
-        match Es !! n' with
-        | Some _ => ε
-        | None => Some ⊤
-        end
-      else
-        ε.
 
-  Definition OwnE_rest u (Es : coPsets) := OwnM (OwnE_restR u Es)%I.
-
-  Definition OwnEs u (Es : coPsets) := ([∗ map] n ↦ E ∈ Es, OwnE u n E)%I.
-
-  Definition OwnE_all u (Es : coPsets) := (OwnE_rest u Es ∗ OwnEs u Es)%I.
-
-  Definition OwnE_top (Es : coPsets) : Prop := map_Forall (fun _ E => ⊤ ⊆ E) Es.
-
-  Definition empty_worldsR {R: world_id -> level -> URA.t} eu (r: forall u n, R u n) :=
-    fun u n =>
+  Definition empty_worldsR {R: univ_id -> URA.t} eu (r: forall u, R u) :=
+    fun u =>
       if (pos_sup eu u)
-      then r u n
+      then r u
       else ε.
 
-  Definition empty_worlds (eu: world_id) : iProp :=
-    OwnM (empty_worldsR eu (fun _ _ => Some ⊤ : CoPset.t) : OwnEsRA)
+  Definition empty_worlds (eu: univ_id) : iProp :=
+    OwnM (empty_worldsR eu (fun _ => Some ⊤ : CoPset.t) : OwnERA)
     ∗
-    OwnM (empty_worldsR eu (fun _ _ => Auth.black (Some ∅ : Gset.t)) : OwnDsRA)
+    OwnM (empty_worldsR eu (fun _ => Auth.black (Some ∅ : Gset.t)) : OwnDRA)
     ∗
-    OwnM (empty_worldsR eu (fun _ n => @Auth.black (_ ==> URA.agree (sProp n))%ra (fun _ => None)) : OwnIsRA sProp)
+    OwnM (empty_worldsR eu (fun _ => (fun n => @Auth.black (_ ==> URA.agree (sProp n))%ra (fun _ => None)) : URA.pointwise_dep _) : OwnIRA sProp)
     .
 
-  Definition free_worlds := (∃ eu, empty_worlds eu)%I.
+  Definition free_universes := (∃ eu, empty_worlds eu)%I.
 
   Definition wsats u b : iProp := ([∗ list] n ∈ (seq 0 b), wsat u n)%I.
 
-  Definition free_auth u b : iProp := OwnD_rest u b ∗ OwnI_rest u b.
+  Definition free_worlds u b : iProp := OwnI_rest u b.
 
-  Definition world u b Es : iProp :=
-    wsats u b ∗ OwnE_all u Es ∗ free_worlds.
+  Definition world u b E : iProp :=
+    wsats u b ∗ OwnE u E ∗ OwnD_auth u ∗ free_universes.
   
-  Definition closed_world u b Es : iProp :=
-    free_auth u b ∗ world u b Es.
-
-  Definition lookup_def (Es : coPsets) n : coPset := default ⊤ (Es !! n).
-
-  Definition subseteq_def (Es : coPsets) n (E : coPset) : Prop :=
-    match Es !! n with | Some E' => E ⊆ E' | None => True end.
-
-  Definition insert_def (Es : coPsets) n : coPsets :=
-    match Es !! n with | Some E => Es | None => <[n:=⊤]> Es end.
+  Definition closed_world u b E : iProp :=
+    free_worlds u b ∗ world u b E.
 
   Lemma unfold_wsats u b :
     wsats u (S b) ⊢ (wsats u b ∗ wsat u b)%I.
@@ -509,12 +458,12 @@ Section WSATS.
     iApply big_sepL_app. ss. iDestruct "A" as "[A B]". iFrame.
   Qed.
 
-  Lemma free_auth_nin_ u (b b' : level) (NIN : b < b')
-    : free_auth u b ⊢ free_auth u b' ∗
-                       ([∗ list] n ∈ (seq b (b' - b)), wsat u n).
+  Lemma free_worlds_nin_ u (b b' : level) (NIN : b < b')
+    : free_worlds u b ⊢ free_worlds u b' ∗
+                      ([∗ list] n ∈ (seq b (b' - b)), wsat u n).
   Proof.
     induction NIN.
-    - iIntros "[DA AUTH]".
+    - iIntros "AUTH".
       assert ((OwnI_restR u b) =
               ((OwnI_restR u (S b))
               ⋅
@@ -540,38 +489,12 @@ Section WSATS.
             rewrite URA.unit_id. reflexivity.
           }
       }
-      assert ((OwnD_restR u b) =
-              ((OwnD_restR u (S b))
-              ⋅
-              (maps_to_res u (maps_to_res b (Auth.black (Some ∅ : Gset.t)))))).
-      { i. subst. extensionalities u' n. unfold OwnD_restR, maps_to_res.
-        do 2 (unfold URA.add; unseal "ra"; ss).
-        destruct (u' =? u)%positive eqn: EQ; cycle 1.
-        { apply Pos.eqb_neq in EQ.
-          destruct (excluded_middle_informative (u' = u)); ss.
-          setoid_rewrite URA.unit_id. eauto.
-        }
-        apply Pos.eqb_eq in EQ. subst.
-        destruct (excluded_middle_informative (u=u)); ss.
-        destruct (excluded_middle_informative (n = b)).
-        - subst n. des_ifs; try lia.
-          unfold eq_rect_r. ss. rewrite URA.unit_idl. reflexivity.
-        - destruct (le_dec n (S b)).
-          { des_ifs; try lia.
-            - rewrite URA.unit_idl. reflexivity.
-            - rewrite URA.unit_id. reflexivity.
-          }
-          { des_ifs; try lia.
-            rewrite URA.unit_id. reflexivity.
-          }
-      }
-      unfold free_auth, OwnD_rest, OwnI_rest.
+      unfold free_worlds, OwnI_rest.
       rewrite H3. iDestruct "AUTH" as "[AUTH NEW]".
-      rewrite H4. iDestruct "DA" as "[DA NEWD]".
-      iPoseProof (wsat_init with "[NEWD NEW]") as "NEW". iFrame.
+      iPoseProof (wsat_init with "NEW") as "NEW". iFrame.
       replace (S b - b) with 1 by lia. ss. iFrame.
-    - unfold free_auth in *.
-      iIntros "[DA AUTH]". iPoseProof (IHNIN with "[DA AUTH]") as "[[DA AUTH] SAT]". iFrame.
+    - unfold free_worlds in *.
+      iIntros "AUTH". iPoseProof (IHNIN with "AUTH") as "[AUTH SAT]". iFrame.
       clear IHNIN.
       assert ((OwnI_restR u m) =
                 ((OwnI_restR u (S m))
@@ -598,51 +521,22 @@ Section WSATS.
             rewrite URA.unit_id. reflexivity.
           }
       }
-      assert ((OwnD_restR u m) =
-              ((OwnD_restR u (S m))
-              ⋅
-              (maps_to_res u (maps_to_res m (Auth.black (Some ∅ : Gset.t)))))).
-      { i. extensionalities u' m'. unfold OwnD_restR, maps_to_res.
-        do 2 (unfold URA.add; unseal "ra"; ss).
-        destruct (u' =? u)%positive eqn: EQ; cycle 1.
-        { apply Pos.eqb_neq in EQ.
-          destruct (excluded_middle_informative (u' = u)); ss.
-          setoid_rewrite URA.unit_id. eauto.
-        }
-        apply Pos.eqb_eq in EQ. subst.
-        destruct (excluded_middle_informative (u=u)); ss.
-        destruct (excluded_middle_informative (m' = m)).
-        - subst. des_ifs; try lia.
-          unfold eq_rect_r. ss. rewrite URA.unit_idl. reflexivity.
-        - destruct (le_dec m' (S m)).
-          { des_ifs; try lia.
-            - rewrite URA.unit_idl. reflexivity.
-            - rewrite URA.unit_id. reflexivity.
-          }
-          { des_ifs; try lia.
-            rewrite URA.unit_id. reflexivity.
-          }
-      }
-      unfold OwnD_rest, OwnI_rest.
+      unfold OwnI_rest.
       rewrite H3. iDestruct "AUTH" as "[AUTH NEW]".
-      rewrite H4. iDestruct "DA" as "[DA NEWD]".
-      iPoseProof (wsat_init with "[NEWD NEW]") as "NEW". iFrame.
-      iSplitL "DA AUTH"; cycle 1. 
-      { iFrame. replace (S m - b) with ((m - b) + 1) by lia. rewrite seq_app.
-        iApply big_sepL_app. iFrame.
-        replace (b + (m - b)) with m by lia. ss. iFrame.
-      }
-      iFrame.
+      iPoseProof (wsat_init with "NEW") as "NEW". iFrame.
+      replace (S m - b) with ((m - b) + 1) by lia. rewrite seq_app.
+      iApply big_sepL_app. iFrame.
+      replace (b + (m - b)) with m by lia. ss. iFrame.
   Qed.
 
-  Lemma free_auth_nin u (b b' : level) (LE : b <= b')
-    : free_auth u b ⊢ free_auth u b' ∗
-                       ([∗ list] n ∈ (seq b (b' - b)), wsat u n).
+  Lemma free_worlds_nin u (b b' : level) (LE : b <= b')
+    : free_worlds u b ⊢ free_worlds u b' ∗
+                      ([∗ list] n ∈ (seq b (b' - b)), wsat u n).
   Proof.
     iIntros "R".
     destruct (le_lt_or_eq _ _ LE); subst; cycle 1.
     - replace (b'-b') with 0 by nia. s. iFrame.
-    - iApply free_auth_nin_; eauto.
+    - iApply free_worlds_nin_; eauto.
   Qed.
 
   Lemma wsats_nin u (b b' : level):
@@ -661,10 +555,10 @@ Section WSATS.
   Qed.
 
   Lemma wsats_allocs u b b':
-    b <= b' -> free_auth u b ∗ wsats u b ⊢ free_auth u b' ∗ wsats u b'.
+    b <= b' -> free_worlds u b ∗ wsats u b ⊢ free_worlds u b' ∗ wsats u b'.
   Proof.
     iIntros (LE) "(AUTH & SAT)".
-    iPoseProof ((free_auth_nin _ _ _ LE) with "AUTH") as "(AUTH & NEW)". iFrame.
+    iPoseProof ((free_worlds_nin _ _ _ LE) with "AUTH") as "(AUTH & NEW)". iFrame.
     iPoseProof ((wsats_nin _ _ _ LE) with "[SAT NEW]") as "SAT". iFrame. iFrame.
   Qed.
 
@@ -674,13 +568,15 @@ Section WSATS.
             | None => True
             | Some G => (exists i, i ∉ G /\ φ i)
             end)
-    : wsats u b ⊢ |==> (∃ i, ⌜φ i⌝ ∧ OwnI u n i p) ∗ (prop n p -∗ wsats u b).
+    : OwnD_auth u ∗ wsats u b ⊢ |==> (∃ i, ⌜φ i⌝ ∧ OwnI u n i p) ∗ OwnD_auth u ∗ (prop n p -∗ wsats u b).
   Proof.
-    iIntros "SALL".
+    iIntros "[DA SALL]".
     iPoseProof (big_sepL_lookup_acc with "SALL") as "[WSAT K]".
     apply lookup_seq_lt; eauto.
-    iPoseProof (wsat_OwnI_alloc_gen with "WSAT") as ">[RES WSAT]". apply INF. iFrame.
-    iModIntro. iIntros "P". iFrame. iPoseProof ("WSAT" with "P") as "WSAT".
+    iPoseProof (wsat_OwnI_alloc_gen with "[DA WSAT]") as ">(RES & DA & WSAT)".
+    { apply INF. } { iFrame. }
+    iFrame. iModIntro. iIntros "P".
+    iPoseProof ("WSAT" with "P") as "WSAT".
     iPoseProof ("K" with "WSAT") as "SALL". iFrame.
   Qed.
 
@@ -690,9 +586,11 @@ Section WSATS.
             | None => True
             | Some G => (exists i, i ∉ G /\ φ i)
             end)
-    : wsats u b ∗ prop n p ⊢ |==> (∃ i, ⌜φ i⌝ ∧ OwnI u n i p) ∗ wsats u b.
+    : OwnD_auth u ∗ wsats u b ∗ prop n p ⊢
+        |==> (∃ i, ⌜φ i⌝ ∧ OwnI u n i p) ∗ OwnD_auth u ∗ wsats u b.
   Proof.
-    iIntros "[W P]". iMod (wsats_OwnI_alloc_lt_gen with "W") as "[I W]". 1,2: eauto.
+    iIntros "(D & W & P)".
+    iMod (wsats_OwnI_alloc_lt_gen with "[D W]") as "(I & D & W)"; eauto. iFrame.
     iModIntro. iFrame. iApply "W". iFrame.
   Qed.
 
@@ -702,13 +600,13 @@ Section WSATS.
             | None => True
             | Some G => (exists i, i ∉ G /\ φ i)
             end)
-    : free_auth u b ∗ wsats u b ⊢        
-                 |==> ((∃ i, ⌜φ i⌝ ∧ OwnI u n i p)
-                         ∗ free_auth u (S n) ∗ (prop n p -∗ wsats u (S n))).
+    : free_worlds u b ∗ OwnD_auth u ∗ wsats u b ⊢ 
+        |==> ((∃ i, ⌜φ i⌝ ∧ OwnI u n i p)
+              ∗ free_worlds u (S n) ∗ OwnD_auth u ∗ (prop n p -∗ wsats u (S n))).
   Proof.
-    iIntros "(AUTH & WSAT)".
+    iIntros "(AUTH & D & WSAT)".
     iPoseProof ((wsats_allocs u b (S n)) with "[AUTH WSAT]") as "[AUTH WSAT]". lia. iFrame.
-    iMod ((wsats_OwnI_alloc_lt_gen u n (S n)) with "WSAT") as "[RES WSAT]". auto. eauto.    
+    iMod ((wsats_OwnI_alloc_lt_gen u n (S n)) with "[D WSAT]") as "[RES WSAT]". auto. eauto. iFrame.
     iModIntro. iFrame.
   Qed.
 
@@ -718,23 +616,23 @@ Section WSATS.
             | None => True
             | Some G => (exists i, i ∉ G /\ φ i)
             end)
-    : free_auth u b ∗ wsats u b ∗ prop n p
-                 ⊢ |==> ((∃ i, ⌜φ i⌝ ∧ OwnI u n i p)
-                           ∗ free_auth u (S n) ∗ wsats u (S n)).
+    : free_worlds u b ∗ OwnD_auth u ∗ wsats u b ∗ prop n p ⊢
+        |==> ((∃ i, ⌜φ i⌝ ∧ OwnI u n i p)
+                ∗ free_worlds u (S n) ∗ OwnD_auth u ∗ wsats u (S n)).
   Proof.
-    iIntros "(A & W & P)". iMod (wsats_OwnI_alloc_ge_gen with "[A W]") as "(I & A & W)".
-    1,2: eauto.
+    iIntros "(A & D & W & P)". iMod (wsats_OwnI_alloc_ge_gen with "[A D W]") as "(I & A & D & W)".
+    1,2: eauto. iFrame.
     iFrame. iModIntro. iFrame. iApply "W". iFrame.
   Qed.
 
-  Lemma free_auth_OwnI_le u b n i p :
-    OwnI u n i p ∗ free_auth u b ⊢ ⌜n < b⌝.
+  Lemma free_worlds_OwnI_le u b n i p :
+    OwnI u n i p ∗ free_worlds u b ⊢ ⌜n < b⌝.
   Proof.
-    iIntros "(I & (_ & AUTH))".
-    unfold OwnI, free_auth, OwnI_rest.
+    iIntros "(I & AUTH)".
+    unfold OwnI, free_worlds, OwnI_rest.
     iCombine "AUTH I" as "AUTH".
     iPoseProof (OwnM_valid with "AUTH") as "%WF".
-    unfold OwnI_restR, maps_to_res, maps_to_res_dep in WF.
+    unfold OwnI_restR, OwnIR, maps_to_res, maps_to_res_dep in WF.
     unfold URA.add in WF. unseal "ra". ss.
     apply (pw_lookup_wf _ u) in WF. ss.
     unfold URA.add in WF. unseal "ra". ss.
@@ -750,7 +648,7 @@ Section WSATS.
   Qed.
 
   Lemma wsats_OwnI_open u b n i p:
-    n < b -> OwnI u n i p ∗ wsats u b ∗ OwnE u n {[i]} ⊢ |==> prop n p ∗ wsats u b ∗ OwnD u n {[i]}.
+    n < b -> OwnI u n i p ∗ wsats u b ∗ OwnE u {[i]} ⊢ |==> prop n p ∗ wsats u b ∗ OwnD u {[i]}.
   Proof.
     iIntros (LT) "(I & SAT & EN)".
     unfold OwnI, wsats.
@@ -762,7 +660,7 @@ Section WSATS.
   Qed.
 
   Lemma wsats_OwnI_close u b n i p:
-    n < b -> OwnI u n i p ∗ wsats u b ∗ prop n p ∗ OwnD u n {[i]} ⊢ |==> wsats u b ∗ OwnE u n {[i]}.
+    n < b -> OwnI u n i p ∗ wsats u b ∗ prop n p ∗ OwnD u {[i]} ⊢ |==> wsats u b ∗ OwnE u {[i]}.
   Proof.
     iIntros (LT) "(I & SAT & P & DIS)".
     iPoseProof (big_sepL_lookup_acc with "SAT") as "[WSAT K]".
@@ -772,204 +670,18 @@ Section WSATS.
     iModIntro. iFrame.
   Qed.
 
-  Lemma OwnE_has u Es n E :
-    (Es !! n = Some E) -> OwnE_all u Es ⊢ OwnE_all u (<[n:=E]>Es).
-  Proof.
-    iIntros (IN) "ES". setoid_rewrite insert_id; auto.
-  Qed.
-
-  Lemma OwnE_alloc u Es n:
-    (Es !! n = None) -> OwnE_all u Es ⊢ |==> OwnE_all u (<[n := ⊤]>Es).
-  Proof.
-    iIntros (NIN) "[AUTH SAT]". unfold OwnE_rest, OwnEs.
-    remember (<[n := ⊤]> Es) as Es'.
-    assert (URA.updatable
-              (OwnE_restR u Es)
-              ((OwnE_restR u Es')
-               ⋅
-               (@maps_to_res _ (_==>_)%ra u (maps_to_res n (Some ⊤))))).
-    { i. do 2 (apply pointwise_updatable; i).
-      unfold OwnE_restR, maps_to_res.
-      do 2 (unfold URA.add; unseal "ra"; ss).
-      destruct (a =? u)%positive eqn: EQ; cycle 1.
-      { apply Pos.eqb_neq in EQ.
-        destruct (excluded_middle_informative (a = u)); ss.
-        setoid_rewrite URA.unit_id. reflexivity. }
-      apply Pos.eqb_eq in EQ. subst.
-      destruct (excluded_middle_informative _); ss.
-      destruct (excluded_middle_informative (a0 = n)).
-      - subst. des_ifs.
-        2:{ exfalso. setoid_rewrite lookup_insert in Heq0. inv Heq0. }
-        rewrite URA.unit_idl. reflexivity.
-      - setoid_rewrite lookup_insert_ne; auto. rewrite URA.unit_id. reflexivity.
-    }
-    iMod (OwnM_Upd H3 with "AUTH") as "[AUTH NEW]". clear H3.
-    iModIntro. unfold OwnE_all, OwnE_rest, OwnEs.
-    iSplitL "AUTH"; eauto.
-    subst. iApply big_sepM_insert; auto. iFrame.
-  Qed.
-
-  Lemma OwnE_acc_in u Es n E (IN : Es !! n = Some E) :
-    OwnE_all u Es ⊢ OwnE u n E ∗ OwnE_all u (<[n := ∅]>Es).
-  Proof.
-    iIntros "[AUTH SAT]". unfold OwnEs.
-    iAssert (OwnE u n E ∗ ([∗ map] n0↦E0 ∈ delete n Es, OwnE u n0 E0))%I with "[SAT]" as "[EN SAT]".
-    { iApply big_sepM_delete; auto. }
-    iPoseProof (OwnM_persistently with "EN") as "#EN2". ss.
-    iAssert ([∗ map] n0↦E0 ∈ <[n := ∅]>Es, OwnE u n0 E0)%I with "[SAT]" as "SAT".
-    { iApply big_sepM_insert_delete. iFrame. iApply (OwnM_extends with "EN2").
-      unfold maps_to_res. clear. exists ε. rewrite URA.unit_id.
-      extensionalities u' n'. des_ifs.
-    }
-    iFrame. iClear "EN2". unfold OwnE_rest.
-    iApply (OwnM_extends with "AUTH"). exists ε. rewrite URA.unit_id.
-    extensionalities u' n'.
-    unfold OwnE_restR. destruct (Nat.eqb_spec n' n).
-    - subst. setoid_rewrite lookup_insert. rewrite IN. auto.
-    - setoid_rewrite lookup_insert_ne; auto.
-  Qed.
-
-  Lemma OwnE_acc_new u Es n (NIN : Es !! n = None) :
-    OwnE_all u Es ⊢ |==> OwnE u n ⊤ ∗ OwnE_all u (<[n := ∅]>Es).
-  Proof.
-    iIntros "ENS". iMod (OwnE_alloc with "ENS") as "ENS". eauto.
-    iModIntro.
-    assert (<[n:=∅]> Es = <[n:=∅]> (<[n:=⊤]> Es)).
-    { setoid_rewrite insert_insert. auto. }
-    rewrite H3. iApply OwnE_acc_in.
-    - setoid_rewrite lookup_insert. auto.
-    - iFrame.
-  Qed.
-
-  Lemma OwnE_all_union u Es n E1 E2 :
-    OwnE_all u (<[n:=E1]> Es) ∗ OwnE u n E2 ⊢ OwnE_all u (<[n:=E1 ∪ E2]> Es).
-  Proof.
-    iIntros "[[AUTH SAT] EN]". unfold OwnE_all. iSplitL "AUTH".
-    {
-      iApply (OwnM_extends with "AUTH"). exists ε. rewrite URA.unit_id.
-      extensionalities u' n'.
-      unfold OwnE_restR. destruct (Nat.eqb_spec n' n).
-      - subst. repeat setoid_rewrite lookup_insert. auto.
-      - repeat setoid_rewrite lookup_insert_ne; auto.
-    }
-    iApply big_sepM_insert_delete.
-    iAssert (OwnE u n E1 ∗ (OwnEs u (delete n (<[n:=E1]> Es))))%I with "[SAT]" as "[EN' SAT]".
-    { iApply big_sepM_delete.
-      - apply lookup_insert.
-      - iFrame.
-    }
-    assert ((delete n (<[n:=E1]> Es)) = delete n Es).
-    { setoid_rewrite delete_insert_delete. auto. }
-    rewrite H3. iFrame. iApply OwnE_union. iFrame.
-  Qed.
-
-  Lemma OwnE_free u Es n :
-    Es !! n = None -> OwnE_all u (<[n:=⊤]>Es) ⊢ |==> OwnE_all u Es.
-  Proof.
-    iIntros (NIN) "ENS". iPoseProof (OwnE_acc_in with "ENS") as "[EN ENS]". apply lookup_insert.
-    rewrite insert_insert. unfold OwnE_all. iDestruct "ENS" as "[AUTH SAT]".
-    iSplitL "EN AUTH".
-    - unfold OwnE_rest, OwnE. iCombine "EN AUTH" as "AUTH".
-      assert (URA.updatable
-                ((maps_to_res u (@maps_to_res level CoPset.t n (Some ⊤)))
-                 ⋅
-                 OwnE_restR u (<[n:=∅]> Es))
-                (OwnE_restR u Es)).
-      { i. do 2 (apply pointwise_updatable; i).
-        unfold OwnE_restR, maps_to_res.
-        do 2 (unfold URA.add; unseal "ra"; ss).
-        destruct (a =? u)%positive eqn: EQ; cycle 1.
-        { apply Pos.eqb_neq in EQ.
-          destruct (excluded_middle_informative (a = u)); ss.
-          setoid_rewrite URA.unit_idl. reflexivity. }
-        apply Pos.eqb_eq in EQ. subst.
-        destruct (excluded_middle_informative _); ss.
-        destruct (excluded_middle_informative (a0 = n)).
-        - subst. rewrite lookup_insert. rewrite NIN.
-          rewrite URA.unit_id. reflexivity.
-        - rewrite lookup_insert_ne; auto. rewrite URA.unit_idl. reflexivity.
-      }
-      iDestruct "AUTH" as "[H AUTH]".
-      iCombine "H AUTH" as "AUTH".
-      iMod (OwnM_Upd H3 with "AUTH") as "AUTH". eauto.
-    - unfold OwnEs. iModIntro.
-      iPoseProof (big_sepM_insert with "SAT") as "[_ SAT]"; auto.
-  Qed.
-
-  Lemma OwnE_update_one u Es n E1 E2 :
-    OwnE_all u (<[n:=E1]>Es) ⊢ (OwnE u n E1 -∗ OwnE u n E2) -∗ OwnE_all u (<[n:=E2]>Es).
-  Proof.
-    iIntros "E IMPL". iPoseProof (OwnE_acc_in with "E") as "[E K]".
-    { apply lookup_insert. }
-    iPoseProof ("IMPL" with "E") as "E".
-    iEval (rewrite insert_insert) in "K".
-    iPoseProof (OwnE_all_union with "[E K]") as "E". iFrame.
-    replace (∅ ∪ E2) with E2 by set_solver.
-    iFrame.
-  Qed.
-
-  Lemma OwnE_all_subset u Es n E1 E2 :
-    (E1 ⊆ E2) -> OwnE_all u (<[n:=E2]>Es) ⊢ OwnE_all u (<[n:=E1]>Es).
-  Proof.
-    iIntros (SUB) "ES". iApply (OwnE_update_one with "ES").
-    iIntros "E". iPoseProof (OwnE_subset with "E") as "[E1 _]". eauto. iFrame.
-  Qed.
-
-  Lemma OwnE_all_disjoint u Es n E1 E2 :
-    E1 ## E2 -> OwnE_all u (<[n:=E1 ∪ E2]>Es) ⊢ OwnE_all u (<[n:=E1]>Es) ∗ OwnE u n E2.
-  Proof.
-    iIntros (HE) "ENS". iPoseProof (OwnE_acc_in with "ENS") as "[EN ENS]".
-    { apply lookup_insert. }
-    iPoseProof ((OwnE_disjoint _ _ _ _ HE) with "EN") as "[EN1 EN2]".
-    iFrame. rewrite insert_insert.
-    iApply (OwnE_update_one with "ENS"). iIntros. iFrame.
-  Qed.
-
-  Lemma OwnE_free_all u Es :
-    OwnE_top Es -> OwnE_all u Es ⊢ |==> OwnE_all u ∅.
-  Proof.
-    pattern Es. revert Es. apply map_ind.
-    { iIntros (TOP) "ES". ss. }
-    iIntros (? ? ? NONE IND TOP) "ES".
-    iMod (OwnE_free with "[ES]") as "ES". eauto.
-    { eapply map_Forall_lookup_1 in TOP. 2: apply lookup_insert. iApply OwnE_all_subset; eauto. }
-    iApply IND. 2: iFrame.
-    eapply map_Forall_insert_1_2; eauto.
-  Qed.
-
-  Lemma OwnE_lookup_def u Es n :
-    OwnE_all u Es ⊢ |==> OwnE_all u (<[n := lookup_def Es n]>Es).
-  Proof.
-    iIntros "ENS". unfold lookup_def, default. des_ifs; ss.
-    - rewrite insert_id; auto.
-    - iMod (OwnE_alloc with "ENS") as "ENS"; eauto.
-  Qed.
-
-  Lemma lookup_subseteq_def Es n E :
-    E ⊆ (lookup_def Es n) -> subseteq_def Es n E.
-  Proof.
-    unfold lookup_def,default, subseteq_def. i. des_ifs.
-  Qed.
-
-  Lemma OwnE_init_wf u:
-    URA.wf (OwnE_restR u ∅).
-  Proof.
-    unfold OwnE_restR. ur. i. ur. i. des_ifs; ur; des_ifs.
-  Qed.
- 
   Lemma empty_worlds_split eu:
-    empty_worlds eu ⊢ (OwnE_all eu ∅ ∗ free_auth eu 0 ∗ empty_worlds (pos_ext_0 eu) ∗ empty_worlds (pos_ext_1 eu)).
+    empty_worlds eu ⊢ free_worlds eu 0 ∗ wsats eu 0 ∗ OwnE eu ⊤ ∗ OwnD_auth eu ∗ empty_worlds (pos_ext_0 eu) ∗ empty_worlds (pos_ext_1 eu).
   Proof.
     assert (ERA: URA.extends
-              ((OwnE_restR eu ∅) ⋅
-               (empty_worldsR (pos_ext_0 eu) (fun _ _ => Some ⊤ : CoPset.t)) ⋅
-               (empty_worldsR (pos_ext_1 eu) (fun _ _ => Some ⊤ : CoPset.t)))
-              (empty_worldsR eu (fun _ _ => Some ⊤ : CoPset.t) : OwnEsRA)).
-    { unfold empty_worldsR, OwnE_restR.
-      exists ε. ur. ur. extensionalities k n.
-      rewrite lookup_empty.
-      destruct (k =? eu)%positive eqn: EQ.
-      { apply Pos.eqb_eq in EQ. subst.
+              ((OwnER eu ⊤) ⋅
+               (empty_worldsR (pos_ext_0 eu) (fun _ => Some ⊤ : CoPset.t)) ⋅
+               (empty_worldsR (pos_ext_1 eu) (fun _ => Some ⊤ : CoPset.t)))
+              (empty_worldsR eu (fun _ => Some ⊤ : CoPset.t) : OwnERA)).
+    { unfold empty_worldsR, OwnER, maps_to_res.
+      exists ε. ur. extensionalities k.
+      destruct (excluded_middle_informative _).
+      { subst. 
         rewrite ->pos_ext_0_sup_false, pos_ext_1_sup_false, pos_sup_refl.
         r_solve. setoid_rewrite URA.unit_id. eauto. }
       destruct (pos_sup (pos_ext_0 eu) k) eqn: SUP0.
@@ -979,19 +691,19 @@ Section WSATS.
       destruct (pos_sup (pos_ext_1 eu) k) eqn: SUP1.
       { erewrite pos_sup_trans; try eassumption; try apply pos_ext_1_sup_true.
         r_solve. setoid_rewrite URA.unit_id. eauto. }
-      rewrite pos_sup_cases; eauto.
-      r_solve.
+      rewrite pos_sup_cases; eauto; r_solve.
+      eapply Pos.eqb_neq; eauto.
     }
 
     assert (DRA: URA.extends
-              ((OwnD_restR eu 0) ⋅
-               (empty_worldsR (pos_ext_0 eu) (fun _ _ => Auth.black (Some ∅ : Gset.t)) : OwnDsRA) ⋅
-               (empty_worldsR (pos_ext_1 eu) (fun _ _ => Auth.black (Some ∅ : Gset.t)) : OwnDsRA))
-              (empty_worldsR eu (fun _ _ => Auth.black (Some ∅ : Gset.t)) : OwnDsRA)).
-    { unfold empty_worldsR, OwnD_restR.
-      exists ε. ur. ur. extensionalities k n.
-      destruct (k =? eu)%positive eqn: EQ.
-      { apply Pos.eqb_eq in EQ. subst.
+              ((OwnD_authR eu ∅) ⋅
+               (empty_worldsR (pos_ext_0 eu) (fun _ => Auth.black (Some ∅ : Gset.t)) : OwnDRA) ⋅
+               (empty_worldsR (pos_ext_1 eu) (fun _ => Auth.black (Some ∅ : Gset.t)) : OwnDRA))
+              (empty_worldsR eu (fun _ => Auth.black (Some ∅ : Gset.t)) : OwnDRA)).
+    { unfold empty_worldsR, OwnD_authR, maps_to_res.
+      exists ε. ur. extensionalities k.
+      destruct (excluded_middle_informative _).
+      { subst.
         rewrite ->pos_ext_0_sup_false, pos_ext_1_sup_false, pos_sup_refl.
         r_solve. setoid_rewrite URA.unit_id. eauto. }
       destruct (pos_sup (pos_ext_0 eu) k) eqn: SUP0.
@@ -1001,79 +713,78 @@ Section WSATS.
       destruct (pos_sup (pos_ext_1 eu) k) eqn: SUP1.
       { erewrite pos_sup_trans; try eassumption; try apply pos_ext_1_sup_true.
         r_solve. setoid_rewrite URA.unit_id. eauto. }
-      rewrite pos_sup_cases; eauto.
-      r_solve.
+      rewrite pos_sup_cases; eauto; r_solve.
+      eapply Pos.eqb_neq; eauto.
     }
 
     assert (IRA: URA.extends
               ((OwnI_restR eu 0) ⋅
-               (empty_worldsR (pos_ext_0 eu) (fun _ n => @Auth.black (_ ==> URA.agree (sProp n))%ra (fun _ => None)) : OwnIsRA sProp) ⋅
-               (empty_worldsR (pos_ext_1 eu) (fun _ n => @Auth.black (_ ==> URA.agree (sProp n))%ra (fun _ => None)) : OwnIsRA sProp))                   
-              (empty_worldsR eu (fun _ n => @Auth.black (_ ==> URA.agree (sProp n))%ra (fun _ => None)) : OwnIsRA sProp)).
+               (empty_worldsR (pos_ext_0 eu) (fun _ => (fun n => @Auth.black (_ ==> URA.agree (sProp n))%ra (fun _ => None)) : URA.pointwise_dep _) : OwnIRA sProp) ⋅
+               (empty_worldsR (pos_ext_1 eu) (fun _ => (fun n => @Auth.black (_ ==> URA.agree (sProp n))%ra (fun _ => None)) : URA.pointwise_dep _) : OwnIRA sProp))
+              (empty_worldsR eu (fun _ => (fun n => @Auth.black (_ ==> URA.agree (sProp n))%ra (fun _ => None)) : URA.pointwise_dep _) : OwnIRA sProp)).
     { unfold empty_worldsR, OwnI_restR.
       exists ε. ur. ur. extensionalities k n.
       destruct (k =? eu)%positive eqn: EQ.
       { apply Pos.eqb_eq in EQ. subst.
         rewrite ->pos_ext_0_sup_false, pos_ext_1_sup_false, pos_sup_refl.
-        r_solve. setoid_rewrite URA.unit_id. eauto. }
+        repeat setoid_rewrite URA.unit_id. eauto. }
       destruct (pos_sup (pos_ext_0 eu) k) eqn: SUP0.
       { rewrite pos_ext_1_disj; eauto.
         erewrite pos_sup_trans; try eassumption; try apply pos_ext_0_sup_true.
-        r_solve. setoid_rewrite URA.unit_id. eauto. }
+        r_solve. repeat setoid_rewrite URA.unit_id. eauto. }
       destruct (pos_sup (pos_ext_1 eu) k) eqn: SUP1.
       { erewrite pos_sup_trans; try eassumption; try apply pos_ext_1_sup_true.
-        r_solve. setoid_rewrite URA.unit_id. eauto. }
+        r_solve. repeat setoid_rewrite URA.unit_id. rewrite URA.add_comm.
+        setoid_rewrite URA.unit_id. eauto. }
       rewrite pos_sup_cases; eauto.
-      r_solve.
+      repeat setoid_rewrite URA.unit_id. r_solve.
     }
 
     iIntros "(ERA & DRA & IRA)".
     iPoseProof ((OwnM_extends ERA) with "ERA") as "[[NE E1] E2]".
     iPoseProof ((OwnM_extends DRA) with "DRA") as "[[ND D1] D2]".
     iPoseProof ((OwnM_extends IRA) with "IRA") as "[[NI I1] I2]".
-    iFrame. unfold OwnEs. rewrite big_sepM_empty. eauto.
+    unfold wsats. s. iFrame.
+    iExists ∅. eauto.
   Qed.
   
   Lemma closed_world_init:
-    empty_worlds 1 ⊢ closed_world 1 0 ∅.
+    empty_worlds 1 ⊢ closed_world 1 0 ⊤.
   Proof.
-    unfold closed_world, world, wsats, free_worlds. s. 
     iIntros "E".
-    iPoseProof (empty_worlds_split with "E") as "(E & DI & R & _)".
+    iPoseProof (empty_worlds_split with "E") as "(F & S & E & D & L & _)".
     iFrame. iExists (pos_ext_0 1). iFrame.
   Qed.
 
-  Lemma closed_world_mon {u} b b' (LE: b <= b') Es:
-    closed_world u b Es ⊢ closed_world u b' Es.
+  Lemma closed_world_mon {u} b b' (LE: b <= b') E:
+    closed_world u b E ⊢ closed_world u b' E.
   Proof.
     unfold closed_world, world, wsats. iIntros "(F & W & E & R)". iFrame.
     replace b' with (b + (b'-b)) by nia.
     rewrite ->seq_app, big_sepL_app. iFrame.
-    iPoseProof (free_auth_nin with "F") as "(FI & W)"; eauto.
+    iPoseProof (free_worlds_nin with "F") as "(FI & W)"; eauto.
     replace (b+(b'-b)) with b' by nia. iFrame.
   Qed.
 
 End WSATS.
 
-Notation "M '!?' k" := (lookup_def M k) (at level 20).
-(* Notation "E '⪿' '(' Es ',' n ')'" := (subseteq_def Es n E) (at level 70). *)
 Section FANCY_UPDATE.
 
   Context `{Σ : GRA.t}.
   Context `{sProp : level -> Type}.
   Context `{Invs : @IInvSet Σ sProp}.
-  Context `{@GRA.inG OwnEsRA Σ}.
-  Context `{@GRA.inG OwnDsRA Σ}.
-  Context `{@GRA.inG (OwnIsRA sProp) Σ}.
+  Context `{@GRA.inG OwnERA Σ}.
+  Context `{@GRA.inG OwnDRA Σ}.
+  Context `{@GRA.inG (OwnIRA sProp) Σ}.
 
   Definition inv u (N : namespace) (n : level) p :=
     (∃ i, ⌜i ∈ (↑N : coPset)⌝ ∧ OwnI u n i p)%I.
 
-  Definition FUpd u b (A : iProp) (Es1 Es2 : coPsets) (P : iProp) : iProp :=
-    A ∗ world u b Es1 -∗ |==> (A ∗ world u b Es2 ∗ P).
+  Definition FUpd u b (A : iProp) (E1 E2 : coPset) (P : iProp) : iProp :=
+    A ∗ world u b E1 -∗ |==> (A ∗ world u b E2 ∗ P).
 
-  Lemma FUpd_mono u b b' A Es1 Es2 P :
-    (b <= b') -> FUpd u b A Es1 Es2 P ⊢ FUpd u b' A Es1 Es2 P.
+  Lemma FUpd_mono u b b' A E1 E2 P :
+    (b <= b') -> FUpd u b A E1 E2 P ⊢ FUpd u b' A E1 E2 P.
   Proof.
     unfold FUpd, world.
     iIntros (LE) "FUPD (A & SAT & EN & R)".
@@ -1082,39 +793,39 @@ Section FANCY_UPDATE.
     iApply wsats_nin. apply LE. iFrame. eauto.
   Qed.
 
-  Lemma wsats_inv_gen u b Es N n p :
+  Lemma wsats_inv_gen u b E N n p :
     n < b ->
-    wsats u b ∗ OwnE_all u Es -∗ |==> inv u N n p ∗ (prop n p -∗ wsats u b) ∗ OwnE_all u Es.
+    wsats u b ∗ OwnE u E ∗ OwnD_auth u -∗ |==> inv u N n p ∗ (prop n p -∗ wsats u b) ∗ OwnE u E ∗ OwnD_auth u.
   Proof.
-    iIntros (LT) "(WSAT & EN)".
-    iMod (wsats_OwnI_alloc_lt_gen _ _ _ LT p (fun i => i ∈ ↑N) with "WSAT") as "(I & WSAT)".
+    iIntros (LT) "(WSAT & EN & DA)".
+    iMod (wsats_OwnI_alloc_lt_gen _ _ _ LT p (fun i => i ∈ ↑N) with "[WSAT DA]") as "(I & D & WSAT)".
     - i. des_ifs. apply iris.base_logic.lib.invariants.fresh_inv_name.
-    - iFrame. auto.
+    - iFrame.
+    - iModIntro. iFrame.
   Qed.
 
-  Lemma FUpd_alloc_gen u b A Es N n p :
-    n < b -> (inv u N n p -∗ prop n p) ⊢ FUpd u b A Es Es (inv u N n p).
+  Lemma FUpd_alloc_gen u b A E N n p :
+    n < b -> (inv u N n p -∗ prop n p) ⊢ FUpd u b A E E (inv u N n p).
   Proof.
-    iIntros (LT) "P (A & W & E & R)".
-    iMod (wsats_inv_gen with "[W E]") as "(#INV & W & E)"; eauto. iFrame.
+    iIntros (LT) "P (A & W & E & D & U)".
+    iMod (wsats_inv_gen with "[W E D]") as "(#INV & W & E)"; eauto. iFrame.
     iPoseProof ("P" with "INV") as "P". iPoseProof ("W" with "P") as "W".
     iModIntro. iFrame. eauto.
   Qed.
 
-  Lemma FUpd_alloc u b A Es N n p :
-    n < b -> prop n p ⊢ FUpd u b A Es Es (inv u N n p).
+  Lemma FUpd_alloc u b A E N n p :
+    n < b -> prop n p ⊢ FUpd u b A E E (inv u N n p).
   Proof.
     iIntros (LT) "P". iApply FUpd_alloc_gen. auto. iIntros. iFrame.
   Qed.
 
-  Lemma FUpd_open_aux u b A Es n N E (LT : n < b) (INE : Es !! n = Some E) (IN : ↑N ⊆ E) p :
+  Lemma FUpd_open u b A n N E (LT : n < b) (IN : ↑N ⊆ E) p :
     inv u N n p ⊢
-        FUpd u b A Es (<[n := E∖↑N]> Es)
-        (prop n p ∗ ((prop n p) -∗ FUpd u b A (<[n := E∖↑N]> Es) Es emp)).
+        FUpd u b A E (E∖↑N)
+        (prop n p ∗ ((prop n p) -∗ FUpd u b A (E∖↑N) E emp)).
   Proof.
-    iIntros "[% (%iN & #HI)] (A & WSAT & ENS & R)".
-    iPoseProof ((OwnE_acc_in _ _ _ _ INE) with "ENS") as "[EN ENS]".
-    iAssert (OwnE u n (E ∖ ↑N) ∗ OwnE u n (↑N ∖ {[i]}) ∗ OwnE u n {[i]})%I with "[EN]" as "(EN1 & EN2 & EN3)".
+    iIntros "[% (%iN & #HI)] (A & WSAT & EN & D & R)".
+    iAssert (OwnE u (E ∖ ↑N) ∗ OwnE u (↑N ∖ {[i]}) ∗ OwnE u {[i]})%I with "[EN]" as "(EN1 & EN2 & EN3)".
     { iApply bi.sep_mono_r.
       { apply OwnE_disjoint. set_solver. }
       iApply OwnE_disjoint.
@@ -1127,182 +838,126 @@ Section FANCY_UPDATE.
     }
     iMod (wsats_OwnI_open _ _ _ i p LT with "[HI WSAT EN3]") as "(P & WSAT & DIS)".
     { iFrame. auto. }
-    iModIntro. iFrame. iPoseProof (OwnE_all_union with "[ENS EN1]") as "ENS". iFrame.
-    replace (∅ ∪ E ∖ ↑N) with (E ∖ ↑N). 2: set_solver.
-    iFrame. iIntros "P (A & WSAT & EN1 & R1)".
+    iModIntro. iFrame.
+    iIntros "P (A & WSAT & EN1 & D1 & R1)".
     iMod (wsats_OwnI_close _ _ _ i p LT with "[HI WSAT P DIS]") as "(WSAT & EN3)".
     { iFrame. auto. }
     iModIntro. iFrame.
     iPoseProof (OwnE_union with "[EN2 EN3]") as "EN2". iFrame.
     rewrite <- union_difference_singleton_L; ss.
-    iPoseProof (OwnE_all_union with "[EN1 EN2]") as "ENS". iFrame.
-    rewrite insert_id. iFrame. rewrite INE. f_equal.
-    rewrite difference_union_L. set_solver.
+    iPoseProof (OwnE_union with "[EN2 EN1]") as "EN". iFrame.
+    rewrite difference_union_L. replace (E ∪ ↑N) with E by set_solver. eauto.
   Qed.
 
-  Lemma FUpd_open u b A Es n N (LT : n < b) (IN : (↑N) ⊆ Es !? n) p :
-    inv u N n p ⊢
-        FUpd u b A Es
-        (<[n := (Es !? n)∖↑N]> Es)
-        ((prop n p) ∗ ((prop n p) -∗ FUpd u b A (<[n := (Es !? n)∖↑N]> Es) Es emp)).
-  Proof.
-    iIntros "[% (%iN & #HI)] (A & WSAT & ENS & R)".
-    unfold lookup_def, subseteq_def in *. destruct (Es !! n) eqn:CASES; ss.
-    - iApply FUpd_open_aux; auto. unfold inv; auto. iFrame.
-    - iAssert (
-          (|==> (A ∗ world u b (<[n:=⊤ ∖ ↑N]> Es) ∗ prop n p ∗ (prop n p -∗ FUpd u b A (<[n:=⊤ ∖ ↑N]> Es) (<[n:=⊤]>Es) emp)))
-          -∗
-          (|==> (A ∗ world u b (<[n:=⊤ ∖ ↑N]> Es) ∗ prop n p ∗ (prop n p -∗ FUpd u b A (<[n:=⊤ ∖ ↑N]> Es) Es emp))))%I as "K".
-      { iIntros ">(A & (SAT & ENS & R) & P & K)". iModIntro. iFrame. iIntros "P".
-        iPoseProof ("K" with "P") as "K". iIntros "(A & SAT & ENS & R)".
-        iPoseProof ("K" with "[A SAT ENS R]") as ">(A & (SAT & ENS & R) & _)". iFrame.
-        iMod (OwnE_free with "ENS") as "ENS". auto.
-        iModIntro. iFrame.
-      }
-      iApply "K". iClear "K".
-      iMod (OwnE_alloc _ _ _ CASES with "ENS") as "ENS". remember (<[n:=⊤]> Es) as Es'.
-      replace (<[n:=⊤ ∖ ↑N]> Es) with (<[n:=⊤ ∖ ↑N]> Es').
-      2:{ subst. rewrite insert_insert. auto. }
-      iApply FUpd_open_aux; auto.
-      { subst. apply lookup_insert. }
-      unfold inv; auto. iFrame.
-  Qed.
-
-  Lemma FUpd_intro u b A Es P :
-    (|==> P) ⊢ FUpd u b A Es Es P.
+  Lemma FUpd_intro u b A E P :
+    (|==> P) ⊢ FUpd u b A E E P.
   Proof.
     iIntros ">P H". iModIntro. iFrame. iFrame.
   Qed.
 
-  Lemma FUpd_mask_frame_gen u b A Es1 Es2 n E P :
-    (Es1 !? n) ## E ->
-    FUpd u b A Es1 Es2 P ⊢
-         FUpd u b A (<[n := (Es1 !? n) ∪ E]>Es1) (<[n := (Es2 !? n) ∪ E]>Es2) P.
-  Proof.
-    rewrite /FUpd. iIntros (D) "H (A & WSAT & ENS & R)".
-    iPoseProof ((OwnE_acc_in _ _ n) with "ENS") as "(EN & ENS)". apply lookup_insert.
-    iPoseProof (OwnE_disjoint _ _ _ _ D with "EN") as "(EN1 & EN)".
-    iPoseProof (OwnE_all_union with "[ENS EN1]") as "ENS". iFrame.
-    replace (∅ ∪ lookup_def Es1 n) with (lookup_def Es1 n) by set_solver.
-    destruct (coPset_equiv_dec E ∅); cycle 1.
-    { unfold lookup_def, default in D. des_ifs; ss.
-      2:{ exfalso. set_solver. }
-      rewrite insert_insert. rewrite (insert_id Es1).
-      2:{ unfold lookup_def, default. rewrite Heq. ss. }
-      iPoseProof ("H" with "[A WSAT ENS R]") as ">(A & (WSAT & ENS2 & R) & P)". iFrame.
-      destruct (Es2 !! n) eqn:CASES.
-      2:{ iMod ((OwnE_acc_new _ _ _ CASES) with "ENS2") as "(EN2 & _)".
-          iPoseProof (OwnE_exploit with "[EN EN2]") as "%DIS". iFrame.
-          set_solver.
-      }
-      unfold lookup_def. rewrite CASES. ss.
-      iPoseProof ((OwnE_acc_in _ _ _ _ CASES) with "ENS2") as "(EN2 & ENS)".
-      iPoseProof (OwnE_union with "[EN EN2]") as "EN". iFrame.
-      iPoseProof (OwnE_all_union with "[ENS EN]") as "ENS". iFrame.
-      replace (∅ ∪ (c0 ∪ E)) with (c0 ∪ E) by set_solver.
-      iModIntro. iFrame.
-    }
-    { replace (lookup_def Es1 n ∪ E) with (lookup_def Es1 n) by set_solver.
-      replace (lookup_def Es2 n ∪ E) with (lookup_def Es2 n) by set_solver.
-      rewrite insert_insert.
-      destruct (Es1 !! n) eqn:CASES.
-      - rewrite (insert_id Es1).
-        2:{ unfold lookup_def, default. rewrite CASES. ss. }
-        iPoseProof ("H" with "[A WSAT ENS R]") as ">(A & (WSAT & ENS2 & R) & P)". iFrame.
-        iMod (OwnE_lookup_def with "ENS2") as "ENS2". iModIntro. iFrame.
-      - replace (lookup_def Es1 n) with (⊤ : coPset).
-        2:{ unfold lookup_def, default. rewrite CASES. ss. }
-        iMod ((OwnE_free _ _ _ CASES) with "ENS") as "ENS".
-        iPoseProof ("H" with "[A WSAT ENS R]") as ">(A & (WSAT & ENS2 & R) & P)". iFrame.
-        iMod (OwnE_lookup_def with "ENS2") as "ENS2". iModIntro. iFrame.
-    }
-  Qed.
-
-  Lemma FUpd_mask_frame u b A Es1 Es2 n E1 E2 E P :
+  Lemma FUpd_mask_frame u b A E1 E2 E P :
     E1 ## E ->
-    FUpd u b A (<[n:=E1]>Es1) (<[n:=E2]>Es2) P ⊢
-         FUpd u b A (<[n :=E1 ∪ E]>Es1) (<[n :=E2 ∪ E]>Es2) P.
+    FUpd u b A E1 E2 P ⊢ FUpd u b A (E1 ∪ E) (E2 ∪ E) P.
   Proof.
-    iIntros (D) "FUPD".
-    iPoseProof (FUpd_mask_frame_gen with "FUPD") as "FUPD".
-    { unfold lookup_def. rewrite lookup_insert. ss. eauto. }
-    unfold lookup_def. rewrite ! lookup_insert. ss. rewrite ! insert_insert. auto.
+    rewrite /FUpd. iIntros (D) "H (A & WSAT & EN & D & R)".
+    iPoseProof (OwnE_disjoint _ _ _ D with "EN") as "(EN1 & EN)".
+    iPoseProof ("H" with "[A WSAT EN1 D R]") as ">(A & (WSAT & EN1 & D & R) & P)". iFrame.
+    iPoseProof (OwnE_union with "[EN EN1]") as "EN". iFrame.
+    iModIntro. iFrame.
   Qed.
 
-  Lemma FUpd_intro_mask u b A Es1 Es2 Es3 n E1 E2 P :
+  Lemma FUpd_intro_mask u b A E1 E2 P :
     E2 ⊆ E1 ->
-    FUpd u b A (<[n:=E1]>Es1) (<[n:=E1]>Es2) P ⊢
-         FUpd u b A (<[n:=E1]>Es1) (<[n:=E2]>Es2) (FUpd u b A (<[n:=E2]>Es3) (<[n:=E1]>Es3) P).
+    FUpd u b A E1 E1 P ⊢ FUpd u b A E1 E2 (FUpd u b A E2 E1 P).
   Proof.
-    rewrite /FUpd. iIntros (HE) "H (A & WSAT & ENS & R)".
-    iPoseProof ("H" with "[A WSAT ENS R]") as ">(A & (WSAT & ENS & R) & P)". iFrame.
-    iModIntro.
-    rewrite (union_difference_L _ _ HE).
-    iPoseProof (OwnE_all_disjoint with "ENS") as "(ENS & EN)".
-    { set_solver. }
-    iFrame. iIntros "(A & WSAT & ENS & R)". iModIntro. iFrame.
-    iApply OwnE_all_union. iFrame.
+    rewrite /FUpd. iIntros (HE) "H (A & WSAT & ENS & D & R)".
+    iPoseProof ("H" with "[A WSAT ENS D R]") as ">(A & (WSAT & ENS & D & R) & P)". iFrame.
+    iModIntro. rewrite (union_difference_L _ _ HE).
+    iPoseProof (OwnE_disjoint with "ENS") as "(ENS & EN)".
+    { set_solver. }    
+    iFrame. iIntros "(A & WSAT & ENS & D & R)". iModIntro. iFrame.
+    iApply OwnE_union. iFrame.
   Qed.
 
-  Lemma FUpd_mask_mono u b A Es1 Es2 n E1 E2 P :
+  Lemma FUpd_mask_mono u b A E1 E2 P :
     E1 ⊆ E2 ->
-    FUpd u b A (<[n:=E1]>Es1) (<[n:=E1]>Es2) P ⊢ FUpd u b A (<[n:=E2]>Es1) (<[n:=E2]>Es2) P.
+    FUpd u b A E1 E1 P ⊢ FUpd u b A E2 E2 P.
   Proof.
     i. replace E2 with (E1 ∪ E2 ∖ E1).
     - eapply FUpd_mask_frame. set_solver.
     - symmetry. eapply leibniz_equiv. eapply union_difference. ss.
   Qed.
 
-  Global Instance from_modal_FUpd u b A Es P :
-    FromModal True modality_id (FUpd u b A Es Es P) (FUpd u b A Es Es P) P.
+  Theorem FUpd_spawn_world u b A E:
+    ⊢ FUpd u b A E E (∃ v, closed_world v 0 ⊤).
+  Proof.
+    unfold FUpd, closed_world, world, free_universes, wsats. s.
+    iIntros "(A & S & E & D & R)". iDestruct "R" as (eu) "EW".
+    iPoseProof (empty_worlds_split with "EW") as "(EW & FA & E' & D' & L' & R')".
+    iFrame. iSplitL "L'"; eauto.
+    iExists eu. iFrame. eauto.
+  Qed.
+
+  Lemma FUpd_send_iprop u b A E u0 b0 E0 N n p
+    (LT: n < b0)
+    :
+    prop n p ∗ closed_world u0 b0 E0
+    ⊢
+    FUpd u b A E E (inv u0 N n p ∗ closed_world u0 b0 E0).
+  Proof.
+    iIntros "(P & F0 & S0 & E0 & D0 & R0) (A & S & E & D & R)".
+    iPoseProof (FUpd_alloc with "P") as "Upd"; eauto.
+    iMod ("Upd" with "[A S0 E0 D0 R0]") as "(A & (S0 & E0 & D9 & R0) & I0)".
+    - iFrame; iAssumption.
+    - iFrame; eauto.
+  Qed.
+
+  Lemma FUpd_receive_iprop u b A E u0 b0 E0 N n p
+    (LT: n < b0)
+    (IN: ↑N ⊆ E0)
+    :
+    inv u0 N n p ∗ closed_world u0 b0 E0
+    ⊢
+    FUpd u b A E E (prop n p ∗ closed_world u0 b0 (E0 ∖↑N)).
+  Proof.
+    iIntros "(I & F0 & S0 & E0 & D0 & R0) (A & S & E & D & R)".
+    iPoseProof (FUpd_open with "I") as "Upd"; eauto.
+    iMod ("Upd" with "[A S0 E0 D0 R0]") as "(A & (S0 & E0 & D0 & R0) & P & _)".
+    - iFrame; iAssumption.
+    - iFrame; eauto.
+  Qed.
+  
+  Global Instance from_modal_FUpd u b A E P :
+    FromModal True modality_id (FUpd u b A E E P) (FUpd u b A E E P) P.
   Proof.
     rewrite /FromModal /= /FUpd. iIntros. iModIntro. iFrame. iFrame.
   Qed.
 
-  Global Instance from_modal_FUpd_alloc u b A Es n P :
-    FromModal (Es !! n = None) modality_id P (FUpd u b A Es (<[n:=⊤]>Es) P) P.
+  Global Instance from_modal_FUpd_general u b A E1 E2 P :
+    FromModal (E2 ⊆ E1) modality_id P (FUpd u b A E1 E2 P) P.
   Proof.
     rewrite /FromModal /FUpd. ss.
-    iIntros (HE) "P (A & WSAT & EN & R)".
-    iMod (OwnE_alloc with "EN") as "EN". eauto. iModIntro. iFrame.
+    iIntros (HE) "P (A & WSAT & EN & D & R)". iModIntro. iFrame.
+    iPoseProof ((OwnE_subset _ _ _ HE) with "EN") as "(EN1 & _)". eauto.
   Qed.
 
-  Global Instance from_modal_FUpd_free u b A Es n P :
-    FromModal (Es !! n = None) modality_id P (FUpd u b A (<[n:=⊤]>Es) Es P) P.
-  Proof.
-    rewrite /FromModal /FUpd. ss.
-    iIntros (HE) "P (A & WSAT & EN & R)".
-    iMod (OwnE_free with "EN") as "EN". eauto. iModIntro. iFrame.
-  Qed.
-
-  Global Instance from_modal_FUpd_general u b A Es n E1 E2 P :
-    FromModal (E2 ⊆ E1) modality_id P (FUpd u b A (<[n:=E1]>Es) (<[n:=E2]>Es) P) P.
-  Proof.
-    rewrite /FromModal /FUpd. ss.
-    iIntros (HE) "P (A & WSAT & EN & R)". iModIntro. iFrame.
-    iPoseProof (OwnE_acc_in with "EN") as "(EN & ENS)". apply lookup_insert.
-    iPoseProof ((OwnE_subset _ _ _ _ HE) with "EN") as "(EN1 & _)".
-    iPoseProof (OwnE_all_union with "[ENS EN1]") as "ENS". iFrame. rewrite insert_insert.
-    replace (∅ ∪ E2) with E2 by set_solver. iFrame.
-  Qed.
-
-  Global Instance from_modal_FUpd_wrong_mask u b A Es1 Es2 P :
+  Global Instance from_modal_FUpd_wrong_mask u b A E1 E2 P :
     FromModal (pm_error "Only non-mask-changing update modalities can be introduced directly.
 Use [FUpd_mask_frame] and [FUpd_intro_mask]")
-              modality_id (FUpd u b A Es1 Es2 P) (FUpd u b A Es1 Es2 P) P | 100.
+              modality_id (FUpd u b A E1 E2 P) (FUpd u b A E1 E2 P) P | 100.
   Proof.
     intros [].
   Qed.
 
-  Global Instance elim_modal_bupd_FUpd p u b A Es1 Es2 P Q :
-    ElimModal True p false (|==> P) P (FUpd u b A Es1 Es2 Q) (FUpd u b A Es1 Es2 Q) | 10.
+  Global Instance elim_modal_bupd_FUpd p u b A E1 E2 P Q :
+    ElimModal True p false (|==> P) P (FUpd u b A E1 E2 Q) (FUpd u b A E1 E2 Q) | 10.
   Proof.
     rewrite /ElimModal bi.intuitionistically_if_elim /FUpd.
     iIntros (_) "(>P & K) I". iApply ("K" with "P"). iFrame.
   Qed.
 
-  Global Instance elim_modal_FUpd_FUpd u p b b' A Es1 Es2 Es3 P Q :
-    ElimModal (b <= b') p false (FUpd u b A Es1 Es2 P) P (FUpd u b' A Es1 Es3 Q) (FUpd u b' A Es2 Es3 Q).
+  Global Instance elim_modal_FUpd_FUpd u p b b' A E1 E2 E3 P Q :
+    ElimModal (b <= b') p false (FUpd u b A E1 E2 P) P (FUpd u b' A E1 E3 Q) (FUpd u b' A E2 E3 Q).
   Proof.
     rewrite /ElimModal bi.intuitionistically_if_elim.
     iIntros (LT) "(P & K) I". inv LT.
@@ -1313,24 +968,25 @@ Use [FUpd_mask_frame] and [FUpd_intro_mask]")
       iMod ("P" with "I") as "(A & (WSAT & EN & R) & P)". iApply ("K" with "P"). iFrame.
   Qed.
 
-  Global Instance elim_modal_FUpd_FUpd_general p u b A Es0 Es1 Es2 n E0 E1 E2 E3 P Q :
+  Global Instance elim_modal_FUpd_FUpd_general p u b A E0 E1 E2 E3 P Q :
     ElimModal (E0 ⊆ E2) p false
-              (FUpd u b A (<[n:=E0]>Es0) (<[n:=E1]>Es1) P)
+              (FUpd u b A E0 E1 P)
               P
-              (FUpd u b A (<[n:=E2]>Es0) (<[n:=E3]>Es2) Q)
-              (FUpd u b A (<[n:=(E1 ∪ (E2 ∖ E0))]>Es1) (<[n:=E3]>Es2) Q) | 10.
+              (FUpd u b A E2 E3 Q)
+              (FUpd u b A (E1 ∪ (E2 ∖ E0)) (E3) Q) | 10.
   Proof.
     rewrite /ElimModal bi.intuitionistically_if_elim. ss.
     iIntros (HE) "[M K]".
-    iPoseProof (FUpd_mask_frame _ _ _ _ _ _ _ _ (E2 ∖ E0) with "M") as "M".
+    iPoseProof (FUpd_mask_frame _ _ _ _ _ (E2 ∖ E0) with "M") as "M".
     { set_solver. }
     replace (E0 ∪ E2 ∖ E0) with E2 by (eapply union_difference_L; ss).
     iMod "M". iPoseProof ("K" with "M") as "M". iFrame.
   Qed.
 
   Global Instance elim_acc_FUpd
-         {X : Type} u b A Es1 Es2 Es (α β : X -> iProp) (mγ : X -> option iProp) (Q : iProp) :
-    ElimAcc True (FUpd u b A Es1 Es2) (FUpd u b A Es2 Es1) α β mγ (FUpd u b A Es1 Es Q) (fun x : X => ((FUpd u b A Es2 Es2 (β x)) ∗ (mγ x -∗? FUpd u b A Es1 Es Q))%I).
+         {X : Type} u b A E1 E2 E (α β : X -> iProp) (mγ : X -> option iProp) (Q : iProp) :
+    ElimAcc True (FUpd u b A E1 E2) (FUpd u b A E2 E1) α β mγ (FUpd u b A E1 E Q)
+      (fun x : X => ((FUpd u b A E2 E2 (β x)) ∗ (mγ x -∗? FUpd u b A E1 E Q))%I).
   Proof.
     iIntros (_) "Hinner >[% [Hα Hclose]]".
     iPoseProof ("Hinner" with "Hα") as "[>Hβ Hfin]".
@@ -1338,10 +994,10 @@ Use [FUpd_mask_frame] and [FUpd_intro_mask]")
     iApply "Hfin". iFrame.
   Qed.
 
-  Global Instance into_acc_FUpd_inv u b A Es n N p :
-    IntoAcc (inv u N n p) (n < b /\ (↑N) ⊆ Es !? n) True
-            (FUpd u b A Es (<[n := Es !? n ∖ ↑N]>Es))
-            (FUpd u b A (<[n := Es !? n ∖ ↑N]>Es) Es)
+  Global Instance into_acc_FUpd_inv u b A E n N p :
+    IntoAcc (inv u N n p) (n < b /\ (↑N) ⊆ E) True
+            (FUpd u b A E (E ∖ ↑N))
+            (FUpd u b A (E ∖ ↑N) E)
             (fun _ : () => prop n p) (fun _ : () => prop n p) (fun _ : () => None).
   Proof.
     rewrite /IntoAcc. iIntros ((LT & iE)) "INV _". rewrite /accessor.
@@ -1349,193 +1005,32 @@ Use [FUpd_mask_frame] and [FUpd_intro_mask]")
     iModIntro. iExists tt. iFrame.
   Qed.
 
-  Global Instance elim_modal_iupd_FUpd p u b A Es1 Es2 P Q :
-    ElimModal True p false (#=(A)=> P) P (FUpd u b A Es1 Es2 Q) (FUpd u b A Es1 Es2 Q) | 10.
+  Global Instance elim_modal_iupd_FUpd p u b A E1 E2 P Q :
+    ElimModal True p false (#=(A)=> P) P (FUpd u b A E1 E2 Q) (FUpd u b A E1 E2 Q) | 10.
   Proof.
     rewrite /ElimModal bi.intuitionistically_if_elim /FUpd.
     iIntros (_) "[P K] [A I]".
     iMod ("P" with "A") as "[A P]". iApply ("K" with "P"). iFrame.
   Qed.
+
+  Global Instance into_acc_FUpd_world u b A E n N p :
+    IntoAcc (inv u N n p) (n < b /\ (↑N) ⊆ E) True
+            (FUpd u b A E (E ∖ ↑N))
+            (FUpd u b A (E ∖ ↑N) E)
+            (fun _ : () => prop n p) (fun _ : () => prop n p) (fun _ : () => None).
+  Proof.
+    rewrite /IntoAcc. iIntros ((LT & iE)) "INV _". rewrite /accessor.
+    iPoseProof (FUpd_open _ _ _ _ _ _ LT iE with "INV") as ">[open close]".
+    iModIntro. iExists tt. iFrame.
+  Qed.
+
+  (* TODO:
+     Needs to register the fancy update rules for multivere operations.
+  *)
   
 End FANCY_UPDATE.
-
-Section MULTIVERSE.
-
-  Context `{Σ : GRA.t}.
-  Context `{sProp : level -> Type}.
-  Context `{Invs : @IInvSet Σ sProp}.
-  Context `{@GRA.inG OwnEsRA Σ}.
-  Context `{@GRA.inG OwnDsRA Σ}.
-  Context `{@GRA.inG (OwnIsRA sProp) Σ}.
-  
-  Theorem spawn_world u b A Es:
-    ⊢ FUpd u b A Es Es (∃ v, closed_world v 0 ∅).
-  Proof.
-    unfold FUpd, closed_world, world, free_worlds, wsats. s.
-    iIntros "(A & S & E & R)". iDestruct "R" as (eu) "EW".
-    iPoseProof (empty_worlds_split with "EW") as "(EW & FA & L & R)".
-    iFrame. iSplitL "L"; eauto.
-    iExists eu. iFrame. eauto.
-  Qed.
-
-  Lemma send_iprop u b A Es u0 b0 Es0 N n p
-    (LT: n < b0)
-    :
-    prop n p ∗ closed_world u0 b0 Es0
-    ⊢
-    FUpd u b A Es Es (inv u0 N n p ∗ closed_world u0 b0 Es0).
-  Proof.
-    iIntros "(P & F0 & S0 & E0 & R0) (A & S & E & R)".
-    iPoseProof (FUpd_alloc with "P") as "Upd"; eauto.
-    iMod ("Upd" with "[A S0 E0 R0]") as "(A & (S0 & E0 & R0) & I0)".
-    iFrame; iAssumption. iFrame; eauto.
-  Qed.
-
-  Lemma receive_iprop u b A Es u0 b0 Es0 N n p
-    (LT: n < b0)
-    (IN: (↑N) ⊆ Es0 !? n)
-    :
-    inv u0 N n p ∗ closed_world u0 b0 Es0
-    ⊢
-    FUpd u b A Es Es (prop n p ∗ closed_world u0 b0 (<[n := (Es0 !? n)∖↑N]> Es0)).
-  Proof.
-    iIntros "(I & F0 & S0 & E0 & R0) (A & S & E & R)".
-    iPoseProof (FUpd_open with "I") as "Upd"; eauto.
-    iMod ("Upd" with "[A S0 E0 R0]") as "(A & (S0 & E0 &R0) & P & _)".
-    iFrame; iAssumption. iFrame; eauto.
-  Qed.  
-
-End MULTIVERSE.
 
 Global Opaque FUpd.
 
 (* Goal (nroot .@ "gil") ## (nroot .@ "hur"). *)
 (* eauto with solve_ndisj. *)
-
-  (* Definition invE := (namespace * { n & sProp n })%type. *)
-
-  (* Definition inv_embed u (e: invE) : iProp := *)
-  (*   inv u e.1 (projT1 e.2) (projT2 e.2). *)
-
-  (* Definition invs_embed u (es: list invE) : iProp := *)
-  (*   [∗ list] e ∈ es, inv_embed u e.     *)
-  
-  (* Fixpoint inv_disj_from (N: namespace) (invs: list invE) : Prop := *)
-  (*   match invs with *)
-  (*   | [] => True *)
-  (*   | (N',_)::invs' => N ## N' /\ inv_disj_from N invs' *)
-  (*   end. *)
-
-  (* Fixpoint inv_disj (invs: list invE) : Prop := *)
-  (*   match invs with *)
-  (*   | [] => True *)
-  (*   | (N,_)::invs' => inv_disj_from N invs' /\ inv_disj invs' *)
-  (*   end. *)
-
-  (* Section TEST. *)
-  (*   Goal forall i, *)
-  (*     inv_disj [(nroot .@ "gil",i); (nroot .@ "hur", i); (nroot .@ "chung", i)]. *)
-  (*   Proof. i. ss.  eauto with solve_ndisj. (* solve_ndisj. *) Qed. *)
-  (* End TEST. *)
-
-  
-(*   Fixpoint invs_in (invs: list invE) Es := *)
-(*     match invs with *)
-(*     | [] => True *)
-(*     | (N, existT n _) :: invs' => *)
-(*         ↑N ⊆ Es !? n ∧ invs_in invs' (<[n := (Es !? n)∖↑N]> Es) *)
-(*     end. *)
-
-(*   Fixpoint invs_remove (invs: list invE) Es := *)
-(*     match invs with *)
-(*     | [] => Es *)
-(*     | (N, existT n _) :: invs' => *)
-(*         invs_remove invs' (<[n := (Es !? n)∖↑N]> Es) *)
-(*     end. *)
-
-  (* Definition update_dep {B: level -> Type} (bs: forall n, B n) (n: level) (b: B n): forall n, B n. *)
-  (*   i. destruct (Nat.eq_dec n0 n); subst. *)
-  (*   - exact b. *)
-  (*   - exact (bs n0). *)
-  (* Defined. *)
-
-  (* Lemma update_dep_eq {B} bs n b : *)
-  (*   @update_dep B bs n b n = b. *)
-  (* Proof. *)
-  (*   unfold update_dep. des_ifs. *)
-  (*   rewrite (UIP _ _ _ e eq_refl). eauto. *)
-  (* Qed. *)
-
-  (* Lemma update_dep_neq {B} bs n b n' *)
-  (*   (NEQ: n <> n') *)
-  (*   : *)
-  (*   @update_dep B bs n b n' = bs n'. *)
-  (* Proof. *)
-  (*   unfold update_dep. des_ifs. *)
-  (* Qed. *)
-
-  (* Lemma big_sepL_seq_exist {B} (unit: forall a, B a) P n sz: *)
-  (*   ([∗ list] a ∈ seq n sz, ∃ b: B a, P a b) *)
-  (*   ⊢ ∃ bs, [∗ list] a ∈ seq n sz, P a (bs a). *)
-  (* Proof. *)
-  (*   revert n. induction sz; ss; i.     *)
-  (*   { iIntros. iExists unit. eauto. } *)
-  (*   iIntros "[NEW SAT]". *)
-  (*   iDestruct "NEW" as (b) "NEW". *)
-  (*   iPoseProof (IHsz with "SAT") as (bs) "SAT". *)
-  (*   iExists (update_dep bs n b). *)
-  (*   iSplitL "NEW". *)
-  (*   { rewrite update_dep_eq. eauto. } *)
-  (*   erewrite big_opL_ext. *)
-  (*   { iApply "SAT". } *)
-  (*   i. s. rewrite update_dep_neq; eauto. *)
-  (*   eapply lookup_seq in H2. des. lia. *)
-  (* Qed. *)
-    
-  (* Lemma big_sepL_seq_exist_rev {B} bs P n sz: *)
-  (*   ([∗ list] a ∈ seq n sz, P a (bs a)) *)
-  (*   ⊢ [∗ list] a ∈ seq n sz, ∃ b: B a, P a b. *)
-  (* Proof. *)
-  (*   revert n. induction sz; ss; i. *)
-  (*   iIntros "[NEW H]". *)
-  (*   iPoseProof (IHsz with "H") as "IH". iFrame. *)
-  (*   iExists (bs n). eauto. *)
-  (* Qed. *)
-
-  (* Lemma OwnE_split u: *)
-  (*   OwnE_all u ∅ ⊢ |==> (OwnE_all (pos_ext_0 u) ∅ ∗ OwnE_all (pos_ext_1 u) ∅). *)
-  (* Proof. *)
-  (*   unfold OwnEs, OwnE_rest, OwnEs, OwnE. *)
-  (*   rewrite !big_sepM_empty. *)
-  (*   assert (URA.updatable (OwnE_restR u ∅) *)
-  (*             ((OwnE_restR (pos_ext_0 u) ∅) ⋅ (OwnE_restR (pos_ext_1 u) ∅))). *)
-  (*   { do 2 (apply pointwise_updatable; i). *)
-  (*     unfold OwnE_restR, maps_to_res. *)
-  (*     do 2 (unfold URA.add; unseal "ra"; ss). *)
-  (*     rewrite lookup_empty. *)
-  (*     destruct (pos_sup (pos_ext_0 u) a) eqn: SUP0. *)
-  (*     { erewrite (pos_sup_trans u _ a); eauto using pos_ext_0_sup_true. *)
-  (*       erewrite pos_ext_1_disj; eauto. *)
-  (*       destruct (a =? pos_ext_1 u)%positive eqn: EQ. *)
-  (*       { apply Pos.eqb_eq in EQ. subst. *)
-  (*         erewrite pos_ext_0_disj in SUP0; ss; eauto using pos_sup_refl. } *)
-  (*       r_solve. des_ifs. *)
-  (*     } *)
-  (*     destruct (pos_sup (pos_ext_1 u) a) eqn: SUP1. *)
-  (*     { erewrite (pos_sup_trans u _ a); eauto using pos_ext_1_sup_true. *)
-  (*       destruct (a =? pos_ext_0 u)%positive eqn: EQ. *)
-  (*       { apply Pos.eqb_eq in EQ. subst. *)
-  (*         erewrite pos_ext_1_disj in SUP1; ss; eauto using pos_sup_refl. } *)
-  (*       r_solve. des_ifs. *)
-  (*     } *)
-  (*     destruct (a =? pos_ext_0 u)%positive eqn: EQ0. *)
-  (*     { apply Pos.eqb_eq in EQ0. subst. rewrite pos_sup_refl in SUP0. ss. } *)
-  (*     destruct (a =? pos_ext_1 u)%positive eqn: EQ1. *)
-  (*     { apply Pos.eqb_eq in EQ1. subst. rewrite pos_sup_refl in SUP1. ss. } *)
-  (*     des_ifs; r_solve; ii; r_solve; *)
-  (*       rewrite URA.add_comm in H2; eapply URA.wf_mon; eauto. *)
-  (*   } *)
-  (*   eapply OwnM_Upd in H2. *)
-  (*   iIntros "[H _]". iPoseProof (H2 with "H") as "H". iMod "H" as "[H1 H2]". *)
-  (*   iFrame. eauto. *)
-  (* Qed. *)
